@prefix cc: <http://web.resource.org/cc/> .
@prefix crm: <http://www.cidoc-crm.org/cidoc-crm/> .
@prefix dcterm: <http://purl.org/dc/terms/> .
@prefix dctype: <http://purl.org/dc/dcmitype/> .
@prefix dul: <http://www.ontologydesignpatterns.org/ont/dul/DUL.owl#> .
@prefix edtf: <http://id.loc.gov/datatypes/edtf/> .
@prefix ev: <http://purl.org/NET/c4dm/event.owl#> .
@prefix foaf: <http://xmlns.com/foaf/0.1/> .
@prefix geo: <http://www.w3.org/2003/01/geo/wgs84_pos#> .
@prefix lode: <http://linkedevents.org/ontology/> .
@prefix owl: <http://www.w3.org/2002/07/owl#> .
@prefix rdf: <http://www.w3.org/1999/02/22-rdf-syntax-ns#> .
@prefix rdfs: <http://www.w3.org/2000/01/rdf-schema#> .
@prefix skos: <http://www.w3.org/2004/02/skos/core#> .
@prefix time: <http://www.w3.org/2006/time#> .
@prefix vann: <http://purl.org/vocab/vann/> .
@prefix xsd: <http://www.w3.org/2001/XMLSchema#> .

<> a owl:Ontology;
dcterm:isVersionOf <http://linkedevents.org/ontology/> ;
dcterm:title "LODE: An ontology for Linking Open Descriptions of Events"@en ;
rdfs:label "LODE: An ontology for Linking Open Descriptions of Events"@en ;
dcterm:issued "2009-10-07"^^xsd:date ;
dcterm:creator [
  foaf:name "Ryan Shaw" ;
  foaf:homepage <http://aeshin.org/> ] ;
dcterm:contributor [
  foaf:name "Raphaël Troncy" ;
  foaf:homepage <http://www.eurecom.fr/~troncy/> ] ;
dcterm:contributor [
  foaf:name "Lynda Hardman" ;
  foaf:homepage <http://www.cwi.nl/~lynda/> ] ;
dcterm:rights "Copyright © 2020 Ryan Shaw" ;
cc:license <http://creativecommons.org/licenses/by-sa/3.0/> ;
rdfs:comment """
This document describes an ontology for publishing descriptions of
historical events as Linked Data, and for mapping between other
event-related vocabularies and ontologies."""@en ;
dcterm:hasFormat <html/>, <ttl/>, <rdfxml/> ;
vann:preferredNamespaceUri "http://linkedevents.org/ontology/" ;
vann:preferredNamespacePrefix "lode" ;
skos:historyNote [
  rdf:value "Added illustrate property." ;
  dcterm:date "2010-10-07"^^xsd:date ;
  dcterm:creator "Raphaël Troncy" ] ;
skos:historyNote [
  rdf:value "Updated CRM and DUL namespaces." ;
  dcterm:date "2020-10-31"^^xsd:date ;
  dcterm:creator "Ryan Shaw" ] ;
skos:changeNote [
  rdf:value "Added Turtle serialization." ;
  dcterm:date "2020-10-31"^^xsd:date ;
  dcterm:creator "Ryan Shaw" ] ;
skos:historyNote [
  rdf:value "Added atEDTFTime property." ;
  dcterm:date "2021-03-28"^^xsd:date ;
  dcterm:creator "Ryan Shaw" ]
.

<html/> dcterm:format [
  a dcterm:IMT;
  rdf:value "text/html" ;
  rdfs:label "HTML"@en ] .

<ttl/> dcterm:format [
  a dcterm:IMT ;
  rdf:value "text/turtle" ;
  rdfs:label "TTL"@en ] .

<rdfxml/> dcterm:format [
  a dcterm:IMT;
  rdf:value "application/rdf+xml" ;
  rdfs:label "RDF/XML"@en ] .

# Classes ----------------------------------------------------------------------

lode:Event a owl:Class;
rdfs:label "Event"@en ;
rdfs:isDefinedBy <http://linkedevents.org/ontology/> ;
dcterm:issued "2009-07-28"^^xsd:date ;
skos:definition """
\"Something that happened,\" as might be reported in a news article or
explained by a historian."""@en ;
rdfs:comment """
An event consists of some temporal and spatial boundaries subjectively
imposed on the flux of reality or imagination, that we wish to treat
as an entity for the purposes of making statements about it. In
particular, we may wish to make statements that relate people, places,
or things to an event."""@en ;
rdfs:comment """
Note that, unlike some defintions of \"event,\" this definition does not
specify that an event involves a change of state, nor does it attempt
to distinguish events from processes or states."""@en ;
.


# Properties  ------------------------------------------------------------------

lode:atTime a owl:ObjectProperty, owl:FunctionalProperty;
rdfs:label "at time"@en ;
rdfs:isDefinedBy <http://linkedevents.org/ontology/> ;
dcterm:issued "2009-07-28"^^xsd:date ;
skos:definition """
an abstract instant or interval of
time that is when an event happened."""@en ;
rdfs:comment """
This property relates an event to some subjectively imposed temporal
boundaries, i.e. a span of time. An event can be related to only one
such span of time."""@en ;
rdfs:comment """
Equivalent definitions from other ontologies:

* C4DM Event ontology: \"Relates an event to a time object, classifying
  a time region (either instantaneous or having an extent).\""""@en ;
rdfs:domain lode:Event;
rdfs:range time:TemporalEntity;
.

lode:atEDTFTime a owl:DatatypeProperty, owl:FunctionalProperty;
rdfs:label "at EDTF time"@en ;
rdfs:isDefinedBy <http://linkedevents.org/ontology/> ;
dcterm:issued "2021-03-28"^^xsd:date ;
skos:definition """
an abstract instant or interval of time that is when an event happened,
expressed as an EDTF literal"""@en ;
rdfs:comment """
This property can be used as an alternative to lode:atTime for
expressing the temporal coverage of an event using the Extended
Date/Time Format (EDTF)."""@en ;
rdfs:domain lode:Event;
rdfs:range edtf:EDTF;
.

lode:circa a owl:ObjectProperty;
rdfs:label "circa"@en ;
rdfs:isDefinedBy <http://linkedevents.org/ontology/> ;
dcterm:issued "2009-07-28"^^xsd:date ;
skos:definition """
an interval of time that can be
precisely described using calendar dates and clock times."""@en ;
rdfs:comment "An temporal relation expressing nearness in time."@en ;
rdfs:comment """
This property relates a span of time that cannot be precisely located
in a chronological series to another span of time that can be
precisely located, thus asserting that the latter is an approximation
of the former."""@en ;
rdfs:domain time:TemporalEntity;
rdfs:range time:DateTimeInterval;
.

lode:inSpace a owl:ObjectProperty, owl:FunctionalProperty;
rdfs:label "in space"@en ;
rdfs:isDefinedBy <http://linkedevents.org/ontology/> ;
dcterm:issued "2009-07-28"^^xsd:date ;
skos:definition """
an abstract region of space (e.g. a
geospatial point or region) that is where an event happened."""@en ;
rdfs:comment """
This property relates an event to some subjectively imposed spatial
boundaries, i.e. a region of space. An event can be related to only
one such region of space."""@en ;
rdfs:comment """
Note that a statement that relates an event to a region of space using
this property only asserts that an event occurred somewhere within
the region and does not assert that it occurred everywhere within the
region."""@en ;
rdfs:domain lode:Event;
rdfs:range geo:SpatialThing;
.

lode:atPlace a owl:ObjectProperty;
rdfs:label "at place"@en ;
rdfs:isDefinedBy <http://linkedevents.org/ontology/> ;
dcterm:issued "2009-07-28"^^xsd:date ;
skos:definition """
a named or relatively specified place that is where
an event happened."""@en ;
rdfs:comment """
This property relates an event to some meaningful place, which may
have a name (e.g. \"Paris\") or may be defined relative to some other
entity or entities (e.g. \"the unincorporated area between Carson and
Harbor Gateway\"). An event may be related to more than one such
place."""@en ;
rdfs:domain lode:Event;
rdfs:range dul:Place;
.

lode:involved a owl:ObjectProperty;
rdfs:label "involved"@en ;
rdfs:isDefinedBy <http://linkedevents.org/ontology/> ;
dcterm:issued "2009-07-28"^^xsd:date ;
skos:definition """
a (physical, social, or mental) object involved in
an event."""@en ;
rdfs:comment """
This property relates an event to any physical, social, or mental
object or substance. It does not imply any causal relationship or
influence or any other kind of explanatory relationship such as
creation, destruction, etc."""@en ;
rdfs:domain lode:Event;
rdfs:range dul:Object;
.

lode:involvedAgent a owl:ObjectProperty;
rdfs:label "involved agent"@en ;
rdfs:isDefinedBy <http://linkedevents.org/ontology/> ;
dcterm:issued "2009-07-28"^^xsd:date ;
skos:definition "an agent involved in an event."@en ;
rdfs:comment """
This property relates an event to anything with agency, such as a
(legal or natural) person, a group, an organization, a computational
agent, etc. It does not imply any causal relationship, influence,
intentionality, etc."""@en ;
rdfs:domain lode:Event;
rdfs:range dul:Agent;
rdfs:subPropertyOf lode:involved;
.

lode:illustrate a owl:ObjectProperty;
rdfs:label "illustrate"@en ;
rdfs:isDefinedBy <http://linkedevents.org/ontology/> ;
dcterm:issued "2010-10-07"^^xsd:date ;
skos:definition """
an event illustrated by some thing (typically a media object)."""@en ;
rdfs:comment """
This property relates any thing (typically a media object) to an event which it
illustrates, documents or comments upon."""@en ;
rdfs:domain owl:Thing;
rdfs:range lode:Event;
.


# Relations with DOLCE+DnS Ultralite ontology ----------------------------------

# The event class and participatory relations have direct equivalents
# in the DOLCE+DnS Ultralite ontology.
lode:Event owl:equivalentClass dul:Event .
lode:involved owl:equivalentProperty dul:hasParticipant .
lode:involvedAgent owl:equivalentProperty dul:involvesAgent .

# lode:atTime is a sub-property of dul:isObservableAt because it
# restricts the domain of the latter to include only events, not all
# entities.
lode:atTime rdfs:subPropertyOf dul:isObservableAt .

# lode:inSpace is a sub-property of dul:hasRegion because it restricts
# the domain of dul:hasRegion to include only events, not all
# entities, and because it restricts the range of dul:hasRegion to
# include only spatial regions, not any dimensional space.
lode:inSpace rdfs:subPropertyOf dul:hasRegion .

# lode:atPlace is a sub-property of dul:hasLocation because it restricts
# the latter such that the domain includes only events (not all
# entities) and the range includes only places (not all entities).
lode:atPlace rdfs:subPropertyOf dul:hasLocation .


# Relations with C4DM Event ontology -------------------------------------------

# The event class, time and space relations, and agent participation
# relation have direct equivalents in the C4DM Event ontology.
lode:Event owl:equivalentClass ev:Event .
lode:atTime owl:equivalentProperty ev:time .
lode:inSpace owl:equivalentProperty ev:place .

# ev:agent is a sub-property of lode:involvedAgent because the latter
# generalizes the former to include all relations to agents whether or
# not their role is "active or "passive".
ev:agent rdfs:subPropertyOf lode:involvedAgent .

# lode:involved is both more specific than ev:factor, because it
# restricts the range of the latter to include only objects, and more
# general, because it does not imply a "passive" role for the involved
# object. Thus there is no equivalence relation between the two.

# There is no property related to ev:product because this ontology
# takes the position that such relationships are better expressed as
# particular views of an event.


# Relations with CIDOC CRM ontology --------------------------------------------

# lode:Event is a sub-class of crm:E2_Temporal_Entity because the latter
# is defined as "anything that happens over a limited extent in time,"
# which is more general than the definition given here. Furthermore,
# the CIDOC CRM documentation specifies that E2_Temporal_Entity is
# "abstract" and "has no direct instances."
lode:Event rdfs:subClassOf crm:E2_Temporal_Entity .

# lode:atTime is a sub-property of crm:P4_has_time-span because it
# restricts the domain of the latter to include only events (as
# defined here) rather than any temporal entity (see above).
lode:atTime rdfs:subPropertyOf crm:P4_has_time-span .

# The following properties generalize properties in the CIDOC CRM
# ontology because they expand the domains of the latter to cover the
# more general definition of event given here.
crm:P7_took_place_at rdfs:subPropertyOf lode:inSpace .
crm:P12_occurred_in_the_presence_of rdfs:subPropertyOf lode:involved .
crm:P11_had_participant rdfs:subPropertyOf lode:involvedAgent .


# Relations with DCMI Type vocabulary ------------------------------------------

# lode:Event is a sub-class of dctype:Event because dctype:Event is an
# rdfs:Class rather than an owl:Class.
lode:Event rdfs:subClassOf dctype:Event .
