<?xml version="1.0" encoding="utf-8"?>
<rdf:RDF xml:base="http://linkedevents.org/ontology/"
  xmlns:skos="http://www.w3.org/2004/02/skos/core#"
  xmlns:dcterm="http://purl.org/dc/terms/"
  xmlns:owl="http://www.w3.org/2002/07/owl#"
  xmlns:vann="http://purl.org/vocab/vann/"
  xmlns:rdf="http://www.w3.org/1999/02/22-rdf-syntax-ns#"
  xmlns:rdfs="http://www.w3.org/2000/01/rdf-schema#"
  xmlns:cc="http://web.resource.org/cc/"
  xmlns:foaf="http://xmlns.com/foaf/0.1/"
>
  <owl:ObjectProperty rdf:about="atPlace">
    <skos:definition xml:lang="en">
a named or relatively specified place that is where
an event happened.</skos:definition>
    <rdfs:domain rdf:resource="Event"/>
    <rdfs:label xml:lang="en">at place</rdfs:label>
    <rdfs:subPropertyOf rdf:resource="http://www.ontologydesignpatterns.org/ont/dul/DUL.owl#hasLocation"/>
    <rdfs:range rdf:resource="http://www.ontologydesignpatterns.org/ont/dul/DUL.owl#Place"/>
    <rdfs:isDefinedBy rdf:resource=""/>
    <rdfs:comment xml:lang="en">
This property relates an event to some meaningful place, which may
have a name (e.g. "Paris") or may be defined relative to some other
entity or entities (e.g. "the unincorporated area between Carson and
Harbor Gateway"). An event may be related to more than one such
place.</rdfs:comment>
    <dcterm:issued rdf:datatype="http://www.w3.org/2001/XMLSchema#date">2009-07-28</dcterm:issued>
  </owl:ObjectProperty>
  <owl:Ontology rdf:about="">
    <dcterm:identifier>http://linkedevents.org/ontology/2021-03-28/</dcterm:identifier>
    <vann:preferredNamespaceUri>http://linkedevents.org/ontology/</vann:preferredNamespaceUri>
    <dcterm:hasFormat rdf:resource="html/"/>
    <dcterm:rights>Copyright © 2021 Ryan Shaw</dcterm:rights>
    <dcterm:isVersionOf rdf:resource=""/>
    <dcterm:modified rdf:datatype="http://www.w3.org/2001/XMLSchema#date">2021-03-28</dcterm:modified>
    <skos:changeNote>
      <rdf:Description rdf:nodeID="ub1bL53C17">
        <dcterm:creator>Ryan Shaw</dcterm:creator>
        <rdf:value>Added Turtle serialization.</rdf:value>
        <dcterm:date rdf:datatype="http://www.w3.org/2001/XMLSchema#date">2020-10-31</dcterm:date>
      </rdf:Description>
    </skos:changeNote>
    <cc:license rdf:resource="http://creativecommons.org/licenses/by-sa/3.0/"/>
    <dcterm:hasFormat rdf:resource="rdfxml/"/>
    <dcterm:date rdf:datatype="http://www.w3.org/2001/XMLSchema#date">2021-03-28</dcterm:date>
    <owl:versionInfo>2021-03-28</owl:versionInfo>
    <rdfs:label xml:lang="en">LODE: An ontology for Linking Open Descriptions of Events</rdfs:label>
    <skos:historyNote>
      <rdf:Description rdf:nodeID="ub1bL57C18">
        <rdf:value>Added atEDTFTime property.</rdf:value>
        <dcterm:creator>Ryan Shaw</dcterm:creator>
        <dcterm:date rdf:datatype="http://www.w3.org/2001/XMLSchema#date">2021-03-28</dcterm:date>
      </rdf:Description>
    </skos:historyNote>
    <dcterm:description xml:lang="en">
This document describes an ontology for publishing descriptions of
historical events as Linked Data, and for mapping between other
event-related vocabularies and ontologies.</dcterm:description>
    <dcterm:creator>
      <rdf:Description rdf:nodeID="ub1bL23C16">
        <foaf:homepage rdf:resource="http://aeshin.org/"/>
        <foaf:name>Ryan Shaw</foaf:name>
      </rdf:Description>
    </dcterm:creator>
    <skos:historyNote>
      <rdf:Description rdf:nodeID="ub1bL45C18">
        <rdf:value>Added illustrate property.</rdf:value>
        <dcterm:creator>Raphaël Troncy</dcterm:creator>
        <dcterm:date rdf:datatype="http://www.w3.org/2001/XMLSchema#date">2010-10-07</dcterm:date>
      </rdf:Description>
    </skos:historyNote>
    <skos:historyNote>
      <rdf:Description rdf:nodeID="ub1bL49C18">
        <dcterm:creator>Ryan Shaw</dcterm:creator>
        <rdf:value>Updated CRM and DUL namespaces.</rdf:value>
        <dcterm:date rdf:datatype="http://www.w3.org/2001/XMLSchema#date">2020-10-31</dcterm:date>
      </rdf:Description>
    </skos:historyNote>
    <dcterm:hasFormat rdf:resource="ttl/"/>
    <dcterm:contributor>
      <rdf:Description rdf:nodeID="ub1bL26C20">
        <foaf:name>Raphaël Troncy</foaf:name>
        <foaf:homepage rdf:resource="http://www.eurecom.fr/~troncy/"/>
      </rdf:Description>
    </dcterm:contributor>
    <dcterm:issued rdf:datatype="http://www.w3.org/2001/XMLSchema#date">2009-10-07</dcterm:issued>
    <dcterm:title xml:lang="en">LODE: An ontology for Linking Open Descriptions of Events</dcterm:title>
    <rdfs:comment xml:lang="en">
This document describes an ontology for publishing descriptions of
historical events as Linked Data, and for mapping between other
event-related vocabularies and ontologies.</rdfs:comment>
    <vann:preferredNamespacePrefix>lode</vann:preferredNamespacePrefix>
    <dcterm:contributor>
      <rdf:Description rdf:nodeID="ub1bL29C20">
        <foaf:homepage rdf:resource="http://www.cwi.nl/~lynda/"/>
        <foaf:name>Lynda Hardman</foaf:name>
      </rdf:Description>
    </dcterm:contributor>
    <dcterm:replaces rdf:resource="2020-10-31/"/>
  </owl:Ontology>
  <owl:FunctionalProperty rdf:about="atTime">
    <rdfs:subPropertyOf rdf:resource="http://www.ontologydesignpatterns.org/ont/dul/DUL.owl#isObservableAt"/>
    <dcterm:issued rdf:datatype="http://www.w3.org/2001/XMLSchema#date">2009-07-28</dcterm:issued>
    <rdfs:comment xml:lang="en">
This property relates an event to some subjectively imposed temporal
boundaries, i.e. a span of time. An event can be related to only one
such span of time.</rdfs:comment>
    <skos:definition xml:lang="en">
an abstract instant or interval of
time that is when an event happened.</skos:definition>
    <rdfs:comment xml:lang="en">
Equivalent definitions from other ontologies:

* C4DM Event ontology: "Relates an event to a time object, classifying
  a time region (either instantaneous or having an extent)."</rdfs:comment>
    <owl:equivalentProperty rdf:resource="http://purl.org/NET/c4dm/event.owl#time"/>
    <rdfs:isDefinedBy rdf:resource=""/>
    <rdfs:subPropertyOf rdf:resource="http://www.cidoc-crm.org/cidoc-crm/P4_has_time-span"/>
    <rdfs:domain rdf:resource="Event"/>
    <rdfs:range rdf:resource="http://www.w3.org/2006/time#TemporalEntity"/>
    <rdfs:label xml:lang="en">at time</rdfs:label>
    <rdf:type rdf:resource="http://www.w3.org/2002/07/owl#ObjectProperty"/>
  </owl:FunctionalProperty>
  <owl:DatatypeProperty rdf:about="atEDTFTime">
    <rdfs:domain rdf:resource="Event"/>
    <dcterm:issued rdf:datatype="http://www.w3.org/2001/XMLSchema#date">2021-03-28</dcterm:issued>
    <rdfs:label xml:lang="en">at EDTF time</rdfs:label>
    <rdfs:range rdf:resource="http://id.loc.gov/datatypes/edtf/EDTF"/>
    <rdfs:isDefinedBy rdf:resource=""/>
    <skos:definition xml:lang="en">
an abstract instant or interval of time that is when an event happened,
expressed as an EDTF literal</skos:definition>
    <rdfs:comment xml:lang="en">
This property can be used as an alternative to lode:atTime for
expressing the temporal coverage of an event using the Extended
Date/Time Format (EDTF).</rdfs:comment>
    <rdf:type rdf:resource="http://www.w3.org/2002/07/owl#FunctionalProperty"/>
  </owl:DatatypeProperty>
  <owl:ObjectProperty rdf:about="illustrate">
    <rdfs:range rdf:resource="Event"/>
    <rdfs:label xml:lang="en">illustrate</rdfs:label>
    <skos:definition xml:lang="en">
an event illustrated by some thing (typically a media object).</skos:definition>
    <rdfs:domain rdf:resource="http://www.w3.org/2002/07/owl#Thing"/>
    <rdfs:comment xml:lang="en">
This property relates any thing (typically a media object) to an event which it
illustrates, documents or comments upon.</rdfs:comment>
    <rdfs:isDefinedBy rdf:resource=""/>
    <dcterm:issued rdf:datatype="http://www.w3.org/2001/XMLSchema#date">2010-10-07</dcterm:issued>
  </owl:ObjectProperty>
  <owl:ObjectProperty rdf:about="circa">
    <skos:definition xml:lang="en">
an interval of time that can be
precisely described using calendar dates and clock times.</skos:definition>
    <dcterm:issued rdf:datatype="http://www.w3.org/2001/XMLSchema#date">2009-07-28</dcterm:issued>
    <rdfs:range rdf:resource="http://www.w3.org/2006/time#DateTimeInterval"/>
    <rdfs:domain rdf:resource="http://www.w3.org/2006/time#TemporalEntity"/>
    <rdfs:isDefinedBy rdf:resource=""/>
    <rdfs:label xml:lang="en">circa</rdfs:label>
    <rdfs:comment xml:lang="en">
This property relates a span of time that cannot be precisely located
in a chronological series to another span of time that can be
precisely located, thus asserting that the latter is an approximation
of the former.</rdfs:comment>
    <rdfs:comment xml:lang="en">An temporal relation expressing nearness in time.</rdfs:comment>
  </owl:ObjectProperty>
  <rdf:Description rdf:about="http://www.cidoc-crm.org/cidoc-crm/P7_took_place_at">
    <rdfs:subPropertyOf rdf:resource="inSpace"/>
  </rdf:Description>
  <rdf:Description rdf:about="http://purl.org/NET/c4dm/event.owl#agent">
    <rdfs:subPropertyOf rdf:resource="involvedAgent"/>
  </rdf:Description>
  <rdf:Description rdf:about="http://www.cidoc-crm.org/cidoc-crm/P11_had_participant">
    <rdfs:subPropertyOf rdf:resource="involvedAgent"/>
  </rdf:Description>
  <rdf:Description rdf:about="http://www.cidoc-crm.org/cidoc-crm/P12_occurred_in_the_presence_of">
    <rdfs:subPropertyOf rdf:resource="involved"/>
  </rdf:Description>
  <owl:Class rdf:about="Event">
    <rdfs:label xml:lang="en">Event</rdfs:label>
    <rdfs:isDefinedBy rdf:resource=""/>
    <rdfs:subClassOf rdf:resource="http://purl.org/dc/dcmitype/Event"/>
    <rdfs:comment xml:lang="en">
An event consists of some temporal and spatial boundaries subjectively
imposed on the flux of reality or imagination, that we wish to treat
as an entity for the purposes of making statements about it. In
particular, we may wish to make statements that relate people, places,
or things to an event.</rdfs:comment>
    <rdfs:comment xml:lang="en">
Note that, unlike some defintions of "event," this definition does not
specify that an event involves a change of state, nor does it attempt
to distinguish events from processes or states.</rdfs:comment>
    <rdfs:subClassOf rdf:resource="http://www.cidoc-crm.org/cidoc-crm/E2_Temporal_Entity"/>
    <owl:equivalentClass rdf:resource="http://purl.org/NET/c4dm/event.owl#Event"/>
    <skos:definition xml:lang="en">
"Something that happened," as might be reported in a news article or
explained by a historian.</skos:definition>
    <dcterm:issued rdf:datatype="http://www.w3.org/2001/XMLSchema#date">2009-07-28</dcterm:issued>
    <owl:equivalentClass rdf:resource="http://www.ontologydesignpatterns.org/ont/dul/DUL.owl#Event"/>
  </owl:Class>
  <owl:ObjectProperty rdf:about="involved">
    <owl:equivalentProperty rdf:resource="http://www.ontologydesignpatterns.org/ont/dul/DUL.owl#hasParticipant"/>
    <rdfs:label xml:lang="en">involved</rdfs:label>
    <rdfs:isDefinedBy rdf:resource=""/>
    <skos:definition xml:lang="en">
a (physical, social, or mental) object involved in
an event.</skos:definition>
    <rdfs:range rdf:resource="http://www.ontologydesignpatterns.org/ont/dul/DUL.owl#Object"/>
    <dcterm:issued rdf:datatype="http://www.w3.org/2001/XMLSchema#date">2009-07-28</dcterm:issued>
    <rdfs:comment xml:lang="en">
This property relates an event to any physical, social, or mental
object or substance. It does not imply any causal relationship or
influence or any other kind of explanatory relationship such as
creation, destruction, etc.</rdfs:comment>
    <rdfs:domain rdf:resource="Event"/>
  </owl:ObjectProperty>
  <rdf:Description rdf:about="ttl/">
    <dcterm:format>
      <dcterm:IMT rdf:nodeID="ub1bL68C22">
        <rdf:value>text/turtle</rdf:value>
        <rdfs:label xml:lang="en">TTL</rdfs:label>
      </dcterm:IMT>
    </dcterm:format>
  </rdf:Description>
  <owl:ObjectProperty rdf:about="inSpace">
    <rdfs:label xml:lang="en">in space</rdfs:label>
    <skos:definition xml:lang="en">
an abstract region of space (e.g. a
geospatial point or region) that is where an event happened.</skos:definition>
    <rdf:type rdf:resource="http://www.w3.org/2002/07/owl#FunctionalProperty"/>
    <dcterm:issued rdf:datatype="http://www.w3.org/2001/XMLSchema#date">2009-07-28</dcterm:issued>
    <owl:equivalentProperty rdf:resource="http://purl.org/NET/c4dm/event.owl#place"/>
    <rdfs:subPropertyOf rdf:resource="http://www.ontologydesignpatterns.org/ont/dul/DUL.owl#hasRegion"/>
    <rdfs:range rdf:resource="http://www.w3.org/2003/01/geo/wgs84_pos#SpatialThing"/>
    <rdfs:domain rdf:resource="Event"/>
    <rdfs:comment xml:lang="en">
Note that a statement that relates an event to a region of space using
this property only asserts that an event occurred somewhere within
the region and does not assert that it occurred everywhere within the
region.</rdfs:comment>
    <rdfs:comment xml:lang="en">
This property relates an event to some subjectively imposed spatial
boundaries, i.e. a region of space. An event can be related to only
one such region of space.</rdfs:comment>
    <rdfs:isDefinedBy rdf:resource=""/>
  </owl:ObjectProperty>
  <rdf:Description rdf:about="rdfxml/">
    <dcterm:format>
      <dcterm:IMT rdf:nodeID="ub1bL73C25">
        <rdfs:label xml:lang="en">RDF/XML</rdfs:label>
        <rdf:value>application/rdf+xml</rdf:value>
      </dcterm:IMT>
    </dcterm:format>
  </rdf:Description>
  <rdf:Description rdf:about="html/">
    <dcterm:format>
      <dcterm:IMT rdf:nodeID="ub1bL63C23">
        <rdf:value>text/html</rdf:value>
        <rdfs:label xml:lang="en">HTML</rdfs:label>
      </dcterm:IMT>
    </dcterm:format>
  </rdf:Description>
  <owl:ObjectProperty rdf:about="involvedAgent">
    <rdfs:range rdf:resource="http://www.ontologydesignpatterns.org/ont/dul/DUL.owl#Agent"/>
    <rdfs:isDefinedBy rdf:resource=""/>
    <dcterm:issued rdf:datatype="http://www.w3.org/2001/XMLSchema#date">2009-07-28</dcterm:issued>
    <rdfs:comment xml:lang="en">
This property relates an event to anything with agency, such as a
(legal or natural) person, a group, an organization, a computational
agent, etc. It does not imply any causal relationship, influence,
intentionality, etc.</rdfs:comment>
    <rdfs:subPropertyOf rdf:resource="involved"/>
    <rdfs:domain rdf:resource="Event"/>
    <rdfs:label xml:lang="en">involved agent</rdfs:label>
    <owl:equivalentProperty rdf:resource="http://www.ontologydesignpatterns.org/ont/dul/DUL.owl#involvesAgent"/>
    <skos:definition xml:lang="en">an agent involved in an event.</skos:definition>
  </owl:ObjectProperty>
</rdf:RDF>
